Change BmapAllocCache rep and prove operations
Like for the DirCache per-directory caches, this uses an optional cache;
if cached data is present, it is assumed correct. Also, an empty and
present cache is now useful; in the previous iteration, an empty cache
meant 'not present, go and fetch'.

The rep is a little convoluted; the problem is that the bottom-level
allocator's rep doesn't special case block 0, even though the actual
allocator function will never return it (see the postcondition for
alloc). Changing the rep would have required an annoying amount of
changes above the block allocator, so instead, the cache rep states that
a present cache is identical to the on-disk state except for block 0,
which is ignored if present in the on-disk state and which can never
appear in the cache.

src/Balloc.v
@@ -1205,14 +1205,14 @@ Module BmapAllocCache (Sig : AllocSig).
   Module Alloc := BmapAlloc Sig.
   Module Defs := Alloc.Defs.
 
-  Definition BmapCacheType := list addr.
+  Definition BmapCacheType := option (list addr).
 
   Record memstate := mk_memstate {
     MSLog  : LOG.memstate;
     MSCache   : BmapCacheType; 
   }.
 
-  Definition freelist0 : BmapCacheType := (@nil addr).
+  Definition freelist0 : BmapCacheType := None.
 
   Definition init lxp xp fms : prog memstate :=
     fms <- Alloc.init lxp xp fms;
@@ -1223,34 +1223,116 @@ Module BmapAllocCache (Sig : AllocSig).
     fms <- Alloc.init_nofree lxp xp ms;
     Ret (mk_memstate fms freelist0).
 
-  Definition alloc lxp xp ms :=
-    let^ (fms, freelist) <- match (MSCache ms) with
-    | nil =>
+  Definition get_free_blocks lxp xp ms :=
+    match (MSCache ms) with
+    | Some x => Ret ^(ms, x)
+    | None =>
       let^ (fms, freelist) <- Alloc.get_free_blocks lxp xp (MSLog ms);
-      Ret ^(fms, freelist)
-    | _ =>
-      Ret ^(MSLog ms, MSCache ms)
-    end;
+      Ret ^((mk_memstate fms (Some freelist)), freelist)
+    end.
+
+  Definition cache_free_block a ms :=
+    match (MSCache ms) with
+    | Some x => Some (a :: x)
+    | None => None
+    end.
+
+  Definition alloc lxp xp (ms : memstate) :=
+    let^ (ms, freelist) <- get_free_blocks lxp xp ms;
     match freelist with
     | nil =>
-      Ret ^((mk_memstate fms freelist), None)
+      Ret ^(ms, None)
     | bn :: freelist' =>
       fms <- Alloc.steal lxp xp bn (MSLog ms);
-      Ret ^((mk_memstate fms freelist'), Some bn)
+      Ret ^((mk_memstate fms (Some freelist')), Some bn)
     end.
 
   Definition free lxp xp bn ms :=
-    fms <- Alloc.free lxp xp bn (MSLog ms) ;
-    Ret (mk_memstate fms (bn ::(MSCache ms))).
+    fms <- Alloc.free lxp xp bn (MSLog ms);
+    let cache := cache_free_block bn ms in
+    Ret (mk_memstate fms cache).
 
   Definition steal lxp xp bn (ms:memstate) :=
     fms <- Alloc.steal lxp xp bn (MSLog ms) ;
     Ret (mk_memstate fms freelist0).
 
+  Definition cache_rep (freelist : list addr) cache :=
+    forall cfreelist, cache = Some cfreelist ->
+    ~In 0 cfreelist /\ NoDup cfreelist /\
+    permutation addr_eq_dec (remove addr_eq_dec 0 freelist) cfreelist.
+
   Definition rep V FP xp freelist (freepred : @pred _ addr_eq_dec V) ms :=
     (Alloc.rep FP xp freelist freepred *
-    [[ incl_count addr_eq_dec (MSCache ms) freelist ]] *
-    [[ forall bn, In bn (MSCache ms) -> bn <> 0 ]])%pred.
+    [[ cache_rep freelist (MSCache ms) ]])%pred.
+
+  Fact cache_rep_freelist0: forall freelist, cache_rep freelist freelist0.
+  Proof.
+    cbv. congruence.
+  Qed.
+
+  Hint Resolve cache_rep_freelist0.
+
+  Lemma cache_rep_remove_cons: forall freelist n cache',
+    cache_rep freelist (Some (n :: cache')) ->
+    cache_rep (remove addr_eq_dec n freelist) (Some cache').
+  Proof.
+    unfold cache_rep. intros.
+    inversion H0; subst.
+    specialize (H _ (eq_refl)). intuition.
+    inversion H; auto.
+    destruct (addr_eq_dec 0 n); subst.
+    cbn in *; intuition auto.
+    rewrite remove_comm.
+    erewrite <- remove_not_In with (l := cfreelist) (a := n).
+    erewrite <- remove_cons with (l := cfreelist).
+    apply permutation_remove; auto.
+    inversion H; auto.
+  Qed.
+
+  Lemma cache_rep_add_cons: forall freelist x cache,
+    cache_rep freelist (Some cache) ->
+    x <> 0 -> ~In x cache ->
+    cache_rep (x :: freelist) (Some (x :: cache)).
+  Proof.
+    unfold cache_rep. intros.
+    specialize (H _ eq_refl).
+    inversion H2; subst.
+    intuition.
+    destruct H4; auto.
+    constructor; auto.
+    rewrite remove_cons_neq by auto.
+    auto using permutation_cons.
+  Qed.
+
+  Lemma cache_rep_in: forall bn freelist cache,
+    cache_rep freelist (Some cache) ->
+    bn <> 0 ->
+    In bn freelist <-> In bn cache.
+  Proof.
+    unfold cache_rep. intros.
+    specialize (H _ eq_refl). intuition.
+    rewrite count_occ_In.
+    rewrite <- H3.
+    rewrite count_occ_remove_ne by auto.
+    rewrite <- count_occ_In. auto.
+    rewrite count_occ_In.
+    erewrite <- count_occ_remove_ne by eauto.
+    rewrite H3.
+    rewrite <- count_occ_In. auto.
+  Qed.
+
+  Lemma cache_rep_none: forall freelist,
+    cache_rep freelist None.
+  Proof.
+    cbv [cache_rep]. intros. congruence.
+  Qed.
+
+  Hint Resolve cache_rep_none.
+
+  Ltac apply_cache_rep := match goal with
+    | Hm: MSCache _ = _, H: cache_rep _ _ |- _ =>
+      rewrite ?Hm in *; specialize (H _ eq_refl) as ?; intuition
+    end.
 
   Theorem init_ok : forall V FP lxp xp ms,
     {< F Fm m0 m bl,
@@ -1290,7 +1372,29 @@ Module BmapAllocCache (Sig : AllocSig).
     step.
   Qed.
 
-  Theorem alloc_ok : forall V FP lxp xp (ms:memstate),
+  Theorem get_free_blocks_ok : forall V FP lxp xp (ms:memstate),
+    {< F Fm m0 m freelist freepred,
+    PRE:hm
+          LOG.rep lxp F (LOG.ActiveTxn m0 m) (MSLog ms) hm *
+          [[[ m ::: (Fm * @rep V FP xp freelist freepred ms) ]]]
+    POST:hm' RET:^(ms, r)
+          [[ MSCache ms = Some r ]] *
+          LOG.rep lxp F (LOG.ActiveTxn m0 m) (MSLog ms) hm' *
+          [[[ m ::: (Fm * @rep V FP xp freelist freepred ms) ]]]
+    CRASH:hm' LOG.intact lxp F m0 hm'
+    >} get_free_blocks lxp xp ms.
+  Proof.
+    unfold get_free_blocks, rep.
+    hoare.
+    rewrite Heqb. auto.
+    unfold cache_rep.
+    intros ? Hs. inversion Hs; intuition subst; auto.
+    auto using permutation_comm.
+  Qed.
+
+  Hint Extern 0 ({{ _ }} Bind (get_free_blocks _ _ _) _) => apply get_free_blocks_ok.
+
+  Theorem alloc_ok : forall V FP lxp xp ms,
     {< F Fm m0 m freelist freepred,
     PRE:hm
           LOG.rep lxp F (LOG.ActiveTxn m0 m) (MSLog ms) hm *
@@ -1306,24 +1410,25 @@ Module BmapAllocCache (Sig : AllocSig).
     CRASH:hm' LOG.intact lxp F m0 hm'
     >} alloc lxp xp ms.
   Proof.
-    unfold alloc, rep; intros.
-    destruct_branch.
+    unfold alloc.
     step.
+    unfold rep in *.
     step.
+    apply_cache_rep.
+    destruct (addr_eq_dec n 0); subst; cbn in *; intuition.
+    rewrite cache_rep_in by eauto.
+    cbn; auto.
     step.
-    eapply In_incl.
-    2: eapply incl_count_incl; eauto.
-    constructor; auto.
-    step.
-    or_r. cancel.
-    apply Alloc.rep_impl_NoDup in H4 as H4'; eauto.
-    apply occ_count_NoDup_impl_NoDup in H9 as H9'; eauto.
-    eapply incl_count_remove_NoDup; eauto.
-    specialize (H8 bn).  apply H8; auto.
-    specialize (H8 n).  apply H8; auto.
+    or_r. cancel; apply_cache_rep.
+    eauto using cache_rep_remove_cons.
+    subst; cbn in *; intuition.
     eapply Alloc.rep_impl_bn_ok with (freelist := freelist); eauto.
-    eapply incl_count_In; eauto.
-    eapply incl_count_In; eauto.
+    eapply remove_still_In.
+    eapply permutation_in; eauto using permutation_comm.
+    cbn; auto.
+    eapply remove_still_In.
+    eapply permutation_in; eauto using permutation_comm.
+    cbn; auto.
   Qed.
 
   Theorem free_ok : forall V FP lxp xp bn ms,
@@ -1342,9 +1447,15 @@ Module BmapAllocCache (Sig : AllocSig).
     >} free lxp xp bn ms.
   Proof.
     unfold free, rep; intros.
+    safestep.
+    eauto.
     step.
-    step.
-    apply incl_count_add; auto.
+    unfold cache_free_block.
+    destruct MSCache eqn:?; auto.
+    eapply cache_rep_add_cons; eauto.
+    assert (NoDup (bn :: freelist)) as Hd by (eauto using Alloc.rep_impl_NoDup).
+    inversion Hd; subst.
+    erewrite <- cache_rep_in by eauto. auto.
   Qed.
 
   Theorem steal_ok : forall V FP lxp xp bn (ms:memstate),
@@ -1361,7 +1472,7 @@ Module BmapAllocCache (Sig : AllocSig).
     >} steal lxp xp bn ms.
   Proof.
     unfold steal, rep; intros.
-    step.
+    safestep.
     step.
   Qed.
 
